Ed: Prove Sha512.Modq

code/experimental/ed25519/Hacl.Impl.SHA512.ModQ.fst
@@ -10,7 +10,7 @@ open Lib.Buffer
 
 module F56 = Hacl.Impl.Ed25519.Field56
 
-#reset-options "--max_fuel 0 --max_ifuel 0"
+#reset-options "--z3rlimit 50 --max_fuel 0 --max_ifuel 0"
 
 //FIX
 val sha512_pre_msg:
@@ -47,14 +47,25 @@ val sha512_pre_pre2_msg:
   Stack unit
     (requires fun h ->
       live h hash /\ live h prefix /\ live h prefix2 /\ live h input /\
-      disjoint prefix hash /\ disjoint prefix2 hash /\ disjoint input hash)
-    (ensures fun h0 _ h1 -> modifies (loc hash) h0 h1)
+      disjoint prefix hash /\ disjoint prefix2 hash /\ disjoint input hash
+    )
+    (ensures fun h0 _ h1 -> modifies (loc hash) h0 h1 /\
+      as_seq h1 hash == Spec.Agile.Hash.hash Spec.Agile.Hash.HASH_SHA2_512
+        (concat #uint8 #64 #(v len)
+          (concat #uint8 #32 #32 (as_seq h0 prefix) (as_seq h0 prefix2))
+          (as_seq h0 input)
+        )
+    )
+
+
 let sha512_pre_pre2_msg h prefix prefix2 len input =
   push_frame ();
   let pre_msg = create (len +. 64ul) (u8 0) in
   assert_norm(pow2 32 <= pow2 125 - 1);
   concat3 32ul prefix 32ul prefix2 len input pre_msg;
+  let h0 = get() in
   Hacl.Hash.SHA2.hash_512 pre_msg (len +. 64ul) h;
+  (**) Hacl.Impl.Hash.Reveal.reveal_agile_sha512 (as_seq h0 pre_msg);
   pop_frame ()
 
 val sha512_modq_pre:
@@ -82,12 +93,10 @@ let sha512_modq_pre out prefix len input =
   push_frame();
   let tmp = create 10ul (u64 0) in
   let hash = create 64ul (u8 0) in
-  let h0 = ST.get() in
   sha512_pre_msg hash prefix len input;
-  let h1 = ST.get() in
   Hacl.Impl.Load56.load_64_bytes tmp hash;
   Hacl.Impl.BignumQ.Mul.barrett_reduction out tmp;
-  admit();
+  assert_norm (pow2 56 == 0x100000000000000);
   pop_frame()
 
 val sha512_modq_pre_pre2:
@@ -123,5 +132,5 @@ let sha512_modq_pre_pre2 out prefix prefix2 len input =
   sha512_pre_pre2_msg hash prefix prefix2 len input;
   Hacl.Impl.Load56.load_64_bytes tmp hash;
   Hacl.Impl.BignumQ.Mul.barrett_reduction out tmp;
-  admit();
+  assert_norm (pow2 56 == 0x100000000000000);
   pop_frame()
